Introduced selectp function to write shortest-path-spec more nicely

formalization/FordFulkerson_Algo.thy
@@ -5,6 +5,54 @@ imports
   Refine_Add_Fofu
   Refine_Monadic_Syntax_Sugar
 begin
+
+  (* TODO: Move to refinement framework. Combine with select from CAVA-Base. *)
+  definition "SELECTp \<equiv> select o Collect"
+
+  lemma selectp_rule[refine_vcg]: 
+    assumes "\<forall>x. \<not>P x \<Longrightarrow> RETURN None \<le> SPEC \<Phi>"
+    assumes "\<And>x. P x \<Longrightarrow> RETURN (Some x) \<le> SPEC \<Phi>"
+    shows "SELECTp P \<le> SPEC \<Phi>"
+    using assms unfolding SELECTp_def select_def[abs_def]
+    by (auto)
+
+  lemma selectp_refine_eq:
+    "SELECTp P \<le> \<Down>(\<langle>R\<rangle>option_rel) (SELECTp Q) \<longleftrightarrow> 
+    (\<forall>x. P x \<longrightarrow> (\<exists>y. (x,y)\<in>R \<and> Q y)) \<and> ((\<forall>x. \<not>P x) \<longrightarrow> (\<forall>y. \<not>Q y))"
+    by (auto simp: SELECTp_def select_def option_rel_def
+      simp: pw_le_iff refine_pw_simps)
+
+  lemma selectp_refine[refine]:
+    assumes "SPEC P \<le>\<Down>R (SPEC Q)"  
+    assumes "\<And>y. \<forall>x. \<not>P x \<Longrightarrow> \<not>Q y"
+    shows "SELECTp P \<le> \<Down>(\<langle>R\<rangle>option_rel) (SELECTp Q)"
+    unfolding selectp_refine_eq
+    using assms by (auto simp: pw_le_iff refine_pw_simps)
+
+  lemma selectp_refine_Id[refine]:  
+    assumes "\<And>x. P x \<Longrightarrow> Q x"
+    assumes "\<And>y. \<forall>x. \<not>P x \<Longrightarrow> \<not>Q y"
+    shows "SELECTp P \<le> \<Down>Id (SELECTp Q)"
+    using selectp_refine[where R=Id, of P Q] assms by auto
+    
+  lemma selectp_pw[refine_pw_simps]:
+    "nofail (SELECTp P)"  
+    "inres (SELECTp P) r \<longleftrightarrow> (r=None \<longrightarrow> (\<forall>x. \<not>P x)) \<and> (\<forall>x. r=Some x \<longrightarrow> P x)"
+    unfolding SELECTp_def select_def[abs_def]
+    by auto
+
+  lemma selectp_pw_simps[simp]:
+    "nofail (SELECTp P)"
+    "inres (SELECTp P) None \<longleftrightarrow> (\<forall>x. \<not>P x)"
+    "inres (SELECTp P) (Some x) \<longleftrightarrow> P x"
+    by (auto simp: refine_pw_simps)
+
+  context Refine_Monadic_Syntax begin 
+    notation SELECTp (binder "selectp " 10)
+
+    term "selectp x. P x"
+  end
+
   text \<open>In this theory, we formalize the abstract Ford-Fulkerson
     method, which is independent of how an augmenting flow is chosen
     \<close>
@@ -17,9 +65,12 @@ begin
       Assuming a valid flow, the procedure must return an augmenting path 
       iff there exists one.
       \<close>
-    definition "find_augmenting_spec f \<equiv> ASSERT (NFlow c s t f) \<guillemotright> 
+    (*definition "find_augmenting_spec f \<equiv> ASSERT (NFlow c s t f) \<guillemotright> 
       SPEC (\<lambda> Some p \<Rightarrow> NFlow.isAugmenting c s t f p 
             | None \<Rightarrow> \<forall>p. \<not>NFlow.isAugmenting c s t f p)"
+    *)
+    definition "find_augmenting_spec f \<equiv> ASSERT (NFlow c s t f) \<guillemotright> 
+      SELECTp (NFlow.isAugmenting c s t f)"
 
     text \<open>
       We also specify the loop invariant, and annotate it to the loop.
@@ -159,7 +210,8 @@ begin
 
     context begin interpretation Refine_Monadic_Syntax .
 
-      private abbreviation "augment \<equiv> NFlow.augment_with_path"
+      private definition "augment \<equiv> NFlow.augment_with_path"
+      private definition "is_augmenting_path f p \<equiv> NFlow.isAugmenting c s t f p"
 
       text \<open>A polished version for presentation\<close>
 (* FIXME: Indentation unfortunate, but required to extract snippet for latex presentation *)    
@@ -170,7 +222,7 @@ definition "ford_fulkerson_algo \<equiv> do {
   (f,_) \<leftarrow> while
     (\<lambda>(f,brk). \<not>brk) 
     (\<lambda>(f,_). do {
-      p \<leftarrow> find_augmenting_spec f;
+      p \<leftarrow> selectp p. is_augmenting_path f p;
       case p of 
         None \<Rightarrow> return (f,True)
       | Some p \<Rightarrow> return (augment c f p, False)
@@ -184,8 +236,9 @@ text_raw \<open>}%EndSnippet\<close>
       proof -
         have "ford_fulkerson_algo \<le> fofu"
           unfolding ford_fulkerson_algo_def fofu_def Let_def
+            find_augmenting_spec_def augment_def is_augmenting_path_def
           apply (rule refine_IdD)
-          apply (refine_rcg)
+          apply (refine_vcg)
           apply (refine_dref_type)
           apply (vc_solve simp: NFlow.augment_with_path_def)
           done
